Polynomial Constant Term via Interpolation

This project computes the constant term of a polynomial by using the interpolation interpretation of the given JSON test cases.

Each JSON entry contains a "base" and a "value".
In this solution, every entry is interpreted as a point on the polynomial:

x = base (read as an integer)

y = value decoded in that base

Using the first k distinct x-values, a unique polynomial of degree k âˆ’ 1 is constructed.
The constant term 
ğ¶
=
ğ‘ƒ
(
0
)
C=P(0) is computed using Lagrange interpolation, evaluated exactly at zero using rational arithmetic.

ğŸ“˜ Testcase 1 â€” Why the Output is -281/6
Input JSON
{
  "keys": { "n": 4, "k": 3 },
  "1": { "base": "10", "value": "4" },
  "2": { "base": "2", "value": "111" },
  "3": { "base": "10", "value": "12" },
  "6": { "base": "4", "value": "213" }
}

Step 1 â€” Convert entries into (x, y) points
JSON key	x = base	value	decoded y
1	10	"4"	4
2	2	"111"	7
3	10	"12"	12 (ignored â€” duplicate x = 10)
6	4	"213"	39

We need k = 3 distinct x-values, so the points are:

(
10
,
4
)
,
 
(
2
,
7
)
,
 
(
4
,
39
)
(10,4), (2,7), (4,39)
Step 2 â€” Compute 
ğ¶
=
ğ‘ƒ
(
0
)
C=P(0) using Lagrange interpolation

General formula:

ğ‘ƒ
(
0
)
=
âˆ‘
ğ‘–
=
1
3
ğ‘¦
ğ‘–
â‹…
â„“
ğ‘–
(
0
)
P(0)=
i=1
âˆ‘
3
	â€‹

y
i
	â€‹

â‹…â„“
i
	â€‹

(0)
â„“
ğ‘–
(
0
)
=
âˆ
ğ‘—
â‰ 
ğ‘–
0
âˆ’
ğ‘¥
ğ‘—
ğ‘¥
ğ‘–
âˆ’
ğ‘¥
ğ‘—
â„“
i
	â€‹

(0)=
j
î€ 
=i
âˆ
	â€‹

x
i
	â€‹

âˆ’x
j
	â€‹

0âˆ’x
j
	â€‹

	â€‹

Term 1: 
(
10
,
4
)
(10,4)
â„“
1
(
0
)
=
âˆ’
2
10
âˆ’
2
â‹…
âˆ’
4
10
âˆ’
4
=
1
6
â„“
1
	â€‹

(0)=
10âˆ’2
âˆ’2
	â€‹

â‹…
10âˆ’4
âˆ’4
	â€‹

=
6
1
	â€‹

4
â‹…
1
6
=
4
6
4â‹…
6
1
	â€‹

=
6
4
	â€‹

Term 2: 
(
2
,
7
)
(2,7)
â„“
2
(
0
)
=
âˆ’
10
2
âˆ’
10
â‹…
âˆ’
4
2
âˆ’
4
=
5
2
â„“
2
	â€‹

(0)=
2âˆ’10
âˆ’10
	â€‹

â‹…
2âˆ’4
âˆ’4
	â€‹

=
2
5
	â€‹

7
â‹…
5
2
=
35
2
=
105
6
7â‹…
2
5
	â€‹

=
2
35
	â€‹

=
6
105
	â€‹

Term 3: 
(
4
,
39
)
(4,39)
â„“
3
(
0
)
=
âˆ’
10
4
âˆ’
10
â‹…
âˆ’
2
4
âˆ’
2
=
âˆ’
5
3
â„“
3
	â€‹

(0)=
4âˆ’10
âˆ’10
	â€‹

â‹…
4âˆ’2
âˆ’2
	â€‹

=âˆ’
3
5
	â€‹

39
â‹…
(
âˆ’
5
3
)
=
âˆ’
65
=
âˆ’
390
6
39â‹…(âˆ’
3
5
	â€‹

)=âˆ’65=âˆ’
6
390
	â€‹

Final Calculation
ğ¶
=
4
6
+
105
6
âˆ’
390
6
=
âˆ’
281
6
C=
6
4
	â€‹

+
6
105
	â€‹

âˆ’
6
390
	â€‹

=
6
âˆ’281
	â€‹

âœ” Final Output for Testcase 1:
âˆ’
281
/
6
âˆ’281/6
	â€‹

ğŸ§ª Testcase 2

The same interpolation method is applied:

decode all base-encoded values,

select the first k distinct x-values,

apply Lagrange interpolation,

evaluate 
ğ‘ƒ
(
0
)
P(0).

This produces another rational constant term (large number), consistent with this interpretation.

ğŸ“ Note on Interpretation

The original problem can also be interpreted as a root-based reconstruction, which leads to completely different results (e.g., 41 for testcase 1).
However, this implementation intentionally uses:

x = base, y = decoded value
âŸ¹
Interpolation
x = base, y = decoded valueâŸ¹Interpolation

This is why the answer differs from solutions using the â€œroots + control pointâ€ formula.